src/3d/prelude/Prelude.fsti
@@ -205,6 +205,50 @@ val parse_string
   (terminator: t)
 : Tot (parser parse_string_kind (cstring t terminator))
 
+inline_for_extraction
+noextract
+let dep_pair_no_terminator_types
+  (#t: eqtype)
+  (terminator: t)
+: Tot (Type u#1)
+=
+  (x: t { x <> terminator }) -> Tot Type0
+
+inline_for_extraction
+noextract
+val sized_list_dep_pair_with_terminator
+  (n: U32.t)
+  (#t: eqtype)
+  (terminator: t)
+  (pl: dep_pair_no_terminator_types terminator)
+: Tot Type0
+
+inline_for_extraction
+noextract
+let dep_pair_no_terminator_parsers
+  (#t: eqtype)
+  (#terminator: t)
+  (#nz: bool)
+  (k: parser_kind nz)
+  (pl: dep_pair_no_terminator_types terminator)
+: Tot Type0
+=
+  (x: t { x <> terminator }) -> Tot (parser k (pl x))
+
+val parse_sized_list_dep_pair_with_terminator
+  (n: U32.t)
+  (#nz: bool)
+  (#kt: parser_kind nz)
+  (#t: eqtype)
+  (pt: parser kt t)
+  (terminator: t)
+  (#nzpl: bool)
+  (#k: parser_kind nzpl)
+  (pl: dep_pair_no_terminator_types terminator)
+  (f: dep_pair_no_terminator_parsers k pl)
+: Tot (parser kind_t_exact (sized_list_dep_pair_with_terminator n terminator pl))
+
+
 ////////////////////////////////////////////////////////////////////////////////
 // Base types
 ////////////////////////////////////////////////////////////////////////////////
